src/extra/Store_Semantics_Extra.v
@@ -1,0 +1,343 @@
+
+(* Extra Lemmas not needed at present *)
+(*
+Lemma unique_store_events: forall t p tr ev1 ev2 loc,
+  well_formed t ->
+  Trace.trace t p tr ->
+  In ev1 tr ->
+  In ev2 tr ->
+  store_event ev1 loc ->
+  store_event ev2 loc ->
+  ev1 <> ev2 ->
+  False.
+Proof.
+  intros.
+  assert (ev1 = ev2).
+  {
+    eapply store_events_injective;
+      try eassumption;
+      try (eapply Trace.trace_events; eassumption).
+  }
+  congruence.
+Defined.
+ *)
+
+(*
+Lemma noDup_store_events: forall t p ev loc tr,
+  well_formed t ->
+  store_event ev loc ->
+  Trace.trace t p tr ->
+  In ev tr ->
+  NoDup ev.
+ *)
+
+(*
+Inductive store_event_evsys: EvSys Ev -> Loc -> Prop :=
+| inevsys_leaf: forall r ev loc,
+    store_event ev loc ->
+    store_event_evsys (leaf r ev) loc
+| inevsys_before_l: forall r es1 es2 loc,
+    store_event_evsys es1 loc ->
+    store_event_evsys (before r es1 es2) loc
+| inevsys_before_r: forall r es1 es2 loc,
+    store_event_evsys es2 loc ->
+    store_event_evsys (before r es1 es2) loc
+| inevsys_merge_l: forall r es1 es2 loc,
+    store_event_evsys es1 loc ->
+    store_event_evsys (merge r es1 es2) loc
+| inevsys_merge_r: forall r es1 es2 loc,
+    store_event_evsys es2 loc ->
+    store_event_evsys (merge r es1 es2) loc.
+Hint Constructors store_event_evsys: core.
+ *)
+
+(*
+Lemma alt_store_event_evsys: forall es loc,
+    store_event_evsys es loc <-> store_event_evsys es loc.
+Proof.
+  intros.
+  unfold store_event_evsys.
+  split.
+  -
+    generalizeEverythingElse es.
+    induction es; intros loc H;
+      inv H;
+      try (eauto; tauto);
+      try ( try (edestruct IHes1; [eauto | destruct_conjs; eauto]; tauto);
+            try (edestruct IHes2; [eauto | destruct_conjs; eauto]; tauto)
+          ).
+  -
+    generalizeEverythingElse es.
+    induction es; intros loc H;
+      destruct H as [x [xx H1]];
+      inv H1; eauto.
+Defined.
+*)
+
+(*
+Lemma aff: forall es1 loc,
+    store_event_evsys es1 loc ->
+    exists ev, store_event ev loc /\ ev_in ev es1.
+Proof.
+  intros.
+  unfold store_event_evsys in *.
+  eauto.
+Defined.
+
+  intros.
+  induction H;
+    try eauto;
+    try (
+        edestruct IHstore_event_evsys;
+        destruct_conjs;
+        exists x;
+        split; eauto).
+Defined.
+ *)
+    
+(*
+
+Inductive top_level_at: (*Plc ->*) Loc -> AnnoTerm -> Prop :=
+(*| top_at_rec: forall r p q loc t',
+          top_level_at q loc t' ->
+          top_level_at p loc (aatt r q t') *)
+| top_at_l: forall q t' loc loc2,
+    top_level_at loc (aatt (loc,loc2) q t')
+| top_at_r: forall q t' loc loc2,
+    top_level_at (pred loc2) (aatt (loc,loc2) q t')
+| top_lseq_l: forall r loc t1 t2,
+    top_level_at loc t1 ->
+    top_level_at loc (alseq r t1 t2)
+| top_lseq_r: forall r loc t1 t2,
+    top_level_at loc t2 ->
+    top_level_at loc (alseq r t1 t2)
+| top_bseq_l: forall r s loc t1 t2,
+    top_level_at loc t1 ->
+    top_level_at loc (abseq r s t1 t2)
+| top_bseq_r: forall r s loc t1 t2,
+    top_level_at loc t2 ->
+    top_level_at loc (abseq r s t1 t2)
+| top_bpar_l: forall r s loc t1 t2,
+    top_level_at loc t1 ->
+    top_level_at loc (abpar r s t1 t2)
+| top_bpar_r: forall r s loc t1 t2,
+    top_level_at loc t2 ->
+    top_level_at loc (abpar r s t1 t2).
+
+Lemma store_event_facts: forall loc t p,
+    store_event_evsys (ev_sys t p) loc ->
+    top_level_at loc t.
+Proof.
+  intros.
+  generalizeEverythingElse t.
+  induction t; intros.
+  -
+    destruct a;
+    
+      inv H;
+        repeat break_let;
+        try solve_by_inversion;
+        inv H0; inv H1.
+  -
+    cbn in *.
+    repeat break_let.
+    invc H.
+    +
+      invc H4.
+      invc H2.
+      econstructor.
+    +
+      invc H4.
+      invc H2.
+      econstructor.
+  -
+    cbn in *.
+    invc H.
+    +
+      econstructor.
+      eauto.
+    +
+      eapply top_lseq_r.
+      eauto.
+  -
+    cbn in *.
+    repeat break_let.
+    invc H.
+    +
+      invc H4.
+      invc H2.
+    +
+      invc H4.
+      ++
+        invc H3.
+        +++
+          econstructor.
+          eauto.
+        +++
+          eapply top_bseq_r.
+          eauto.
+      ++
+        invc H3.
+        invc H2.
+  -
+    cbn in *.
+    repeat break_let.
+    invc H.
+    +
+      invc H4.
+      invc H2.
+    +
+      invc H4.
+      ++
+        invc H3.
+        +++
+          econstructor.
+          eauto.
+        +++
+          eapply top_bpar_r.
+          eauto.
+      ++
+        invc H3.
+        invc H2.
+Defined.
+
+Lemma wf_att_fact: forall x y q t',
+    well_formed (aatt (x, y) q t') ->
+    x > (Nat.pred y) ->
+    False.
+Proof.
+  intros.
+  inv H.
+  simpl in *.
+  lia.
+Defined.
+
+Lemma good_par : forall r s p t1 t2 loc,
+    well_formed (abpar r s t1 t2) ->
+    store_event_evsys (ev_sys t1 p) loc ->
+    store_event_evsys (ev_sys t2 p) loc ->
+    False.
+Proof.
+  intros.
+  eapply store_event_facts in H0.
+  eapply store_event_facts in H1.
+  inv H.
+  Check anno_mono.
+  inv H0; inv H1; cbn in *.
+
+  invc H0; invc H1;
+    try lia.
+
+  invc H0; invc H1;
+    try lia.
+
+  eapply wf_att_fact.
+  apply H7.
+  lia.
+
+  rewrite <- H3 in *.
+  subst.
+  invc H7.
+  simpl in *.
+  lia.
+
+
+  
+
+  invc H6.
+  simpl in *.
+  subst.
+
+  invc H0; try lia.
+  pose (wf_mono t' H12).
+  simpl in *.
+  subst.
+  rewrite <- H13 in *.
+  rewrite H14 in *.
+  simpl in *.
+  destruct (range t') eqn:hey.
+  simpl in *.
+  subst.
+  destruct r.
+  simpl in *.
+  subst.
+  destruct r0.
+  simpl in *.
+  subst.
+  clear H1.
+  invc H7.
+  subst.
+
+  simpl in *.
+  subst.
+  pose (wf_mono t1 H4).
+  subst.
+  rewrite H8 in *.
+  subst.
+  rewrite <- H6 in *; clear H6.
+  rewrite <- H8 in *; clear H8.
+  
+  subst.
+  admit.
+  
+Admitted.
+
+ *)
+
+(*
+
+
+Theorem no_store_conflicts: forall t p,
+    well_formed t ->
+    not (store_conflict (ev_sys t p)).
+Proof.
+  Print ev_sys.
+  unfold not; intros.
+  generalize dependent p.
+  induction t; intros.
+  -
+    destruct a;
+      try (inv H0; repeat break_let; solve_by_inversion).
+  -
+    cbn in *.
+    repeat break_let.
+    invc H0.
+    +
+      solve_by_inversion.
+    +
+      solve_by_inversion.
+  -
+    inv H.
+    invc H0; eauto.
+  -
+    inv H.
+    invc H0;
+      repeat break_let;
+      try solve_by_inversion.
+    +
+      invc H1.
+      solve_by_inversion.
+    +
+      invc H1.
+      invc H2.
+      ++
+        invc H1; eauto.
+      ++
+        solve_by_inversion.
+  -
+    inv H.
+    invc H0;
+      repeat break_let;
+      try solve_by_inversion.
+    +
+      invc H1.
+      solve_by_inversion.
+    +
+      invc H1.
+      invc H2; try solve_by_inversion.
+      invc H1.
+      
+      eapply good_par; eauto.
+Defined.
+  
+  *)
